finished section 3.5

analysis/Analysis/Section_3_5.lean
@@ -51,31 +51,45 @@ theorem OrderedPair.eq (x y x' y' : Object) :
 
 /-- Helper lemma for Exercise 3.5.1 -/
 lemma SetTheory.Set.pair_eq_singleton_iff {a b c: Object} : {a, b} = ({c}: Set) ↔
-    a = c ∧ b = c := by
-  sorry
+  a = c ∧ b = c := by
+    constructor
+    · intro h
+      replace h := Set.ext_iff.mp h
+      exact ⟨
+        h a |>.mp (mem_pair _ _ _ |>.mpr (Or.inl rfl)) |> (mem_singleton _ _ |>.mp),
+        h b |>.mp (mem_pair _ _ _ |>.mpr (Or.inr rfl)) |> (mem_singleton _ _ |>.mp)
+      ⟩
+    rintro ⟨rfl, rfl⟩ 
+    exact pair_self _
 
+
+open SetTheory in
 /-- Exercise 3.5.1, first part -/
 def OrderedPair.toObject : OrderedPair ↪ Object where
   toFun p := ({ (({p.fst}:Set):Object), (({p.fst, p.snd}:Set):Object) }:Set)
-  inj' := by sorry
+  inj' := by
+    rintro ⟨a1, a2⟩ ⟨b1, b2⟩ h
+    simp_all
+    obtain ⟨h1,h2⟩|⟨h1,h2⟩ := pair_eq_iff.mp h
+    all_goals
+      clear h
+      apply Function.Embedding.injective set_to_object at h1
+      apply Function.Embedding.injective set_to_object at h2
+    · obtain rfl := singleton_eq_iff.mp h1
+      obtain rfl := pair_eq_iff'.mp h2
+      exact ⟨rfl, rfl⟩ 
+    · replace h1 := pair_eq_singleton_iff.mp h1.symm
+      replace h2 := pair_eq_singleton_iff.mp h2
+      refine ⟨h1.left.symm, h2.right.trans h1.left |>.trans h1.right.symm⟩ 
 
 instance OrderedPair.inst_coeObject : Coe OrderedPair Object where
   coe := toObject
 
-/--
-  A technical operation, turning a object `x` and a set `Y` to a set `{x} × Y`, needed to define
-  the full Cartesian product
--/
-abbrev SetTheory.Set.slice (x:Object) (Y:Set) : Set :=
-  Y.replace (P := fun y z ↦ z = (⟨x, y⟩:OrderedPair)) (by grind)
-
-@[simp]
-theorem SetTheory.Set.mem_slice (x z:Object) (Y:Set) :
-    z ∈ (SetTheory.Set.slice x Y) ↔ ∃ y:Y, z = (⟨x, y⟩:OrderedPair) := replacement_axiom _ _
-
 /-- Definition 3.5.4 (Cartesian product) -/
 abbrev SetTheory.Set.cartesian (X Y:Set) : Set :=
-  union (X.replace (P := fun x z ↦ z = slice x Y) (by grind))
+  union (X.replace (P := fun x z ↦ z = 
+    Y.replace (P := fun y z ↦ z = (⟨x, y⟩:OrderedPair)) (by grind)
+  ) (by grind))
 
 /-- This instance enables the ×ˢ notation for Cartesian product. -/
 instance SetTheory.Set.inst_SProd : SProd Set Set Set where
@@ -89,8 +103,32 @@ theorem SetTheory.Set.mem_cartesian (z:Object) (X Y:Set) :
   simp only [SProd.sprod, union_axiom]; constructor
   . intro ⟨ S, hz, hS ⟩; rw [replacement_axiom] at hS; obtain ⟨ x, hx ⟩ := hS
     use x; simp_all
-  rintro ⟨ x, y, rfl ⟩; use slice x Y; refine ⟨ by simp, ?_ ⟩
+  rintro ⟨ x, y, rfl ⟩
+  use Y.replace (P := fun y z ↦ z = (⟨x, y⟩:OrderedPair)) (by grind)
+  refine ⟨ by simp, ?_ ⟩
   rw [replacement_axiom]; use x
+
+@[simp]
+theorem SetTheory.Set.cartesian_empty_iff { X Y:Set } :
+  X ×ˢ Y = ∅ ↔ X = ∅ ∨ Y = ∅ := by
+    simp_rw [eq_empty_iff_forall_notMem, mem_cartesian, not_exists]
+    constructor
+    · intro h
+      by_contra! h'
+      obtain ⟨⟨x, hx⟩, ⟨y, hy⟩⟩ := h'
+      apply h (OrderedPair.mk x y) ⟨x, hx⟩ ⟨y, hy⟩  
+      rfl
+    rintro (h|h) x f s
+    exact absurd f.prop (h f.val) 
+    exact absurd s.prop (h s.val) 
+
+@[simp]
+theorem SetTheory.Set.cartesian_nonempty_iff { X Y:Set } :
+  X ×ˢ Y ≠ ∅ ↔ X ≠ ∅ ∧ Y ≠ ∅ := by
+    apply not_iff_not.mp
+    rw [Classical.not_and_iff_not_or_not]
+    push_neg
+    exact cartesian_empty_iff
 
 noncomputable abbrev SetTheory.Set.fst {X Y:Set} (z:X ×ˢ Y) : X :=
   ((mem_cartesian _ _ _).mp z.property).choose
@@ -152,17 +190,17 @@ example : ({1, 2}: Set) ×ˢ ({3, 4, 5}: Set) = ({
 
 /-- Example 3.5.5 / Exercise 3.6.5. There is a bijection between `X ×ˢ Y` and `Y ×ˢ X`. -/
 noncomputable abbrev SetTheory.Set.prod_commutator (X Y:Set) : X ×ˢ Y ≃ Y ×ˢ X where
-  toFun := sorry
-  invFun := sorry
-  left_inv := sorry
-  right_inv := sorry
+  toFun z := mk_cartesian (snd z) (fst z)
+  invFun z := mk_cartesian (snd z) (fst z)
+  left_inv z := by simp
+  right_inv z := by simp
 
 /-- Example 3.5.5. A function of two variables can be thought of as a function of a pair. -/
 noncomputable abbrev SetTheory.Set.curry_equiv {X Y Z:Set} : (X → Y → Z) ≃ (X ×ˢ Y → Z) where
   toFun f z := f (fst z) (snd z)
-  invFun f x y := f ⟨ (⟨ x, y ⟩:OrderedPair), by simp ⟩
+  invFun f x y := f (mk_cartesian x y)
   left_inv _ := by simp
-  right_inv _ := by simp [←pair_eq_fst_snd]
+  right_inv _ := by simp
 
 /-- Definition 3.5.6.  The indexing set `I` plays the role of `{ i : 1 ≤ i ≤ n }` in the text.
     See Exercise 3.5.10 below for some connections betweeen this concept and the preceding notion
@@ -188,7 +226,14 @@ theorem SetTheory.Set.tuple_mem_iProd {I: Set} {X: I → Set} (x: ∀ i, X i) :
 
 @[simp]
 theorem SetTheory.Set.tuple_inj {I:Set} {X: I → Set} (x y: ∀ i, X i) :
-    tuple x = tuple y ↔ x = y := by sorry
+  tuple x = tuple y ↔ x = y := by
+    refine ⟨?_, fun h => h ▸ rfl⟩ 
+    intro h
+    funext i
+    rw [coe_of_fun_inj, funext_iff] at h
+    replace h := Subtype.mk.injEq _ _ _ _ ▸ h i
+    exact (coe_inj _ _ _).mp h
+
 
 /-- Example 3.5.8. There is a bijection between `(X ×ˢ Y) ×ˢ Z` and `X ×ˢ (Y ×ˢ Z)`. -/
 noncomputable abbrev SetTheory.Set.prod_associator (X Y Z:Set) : (X ×ˢ Y) ×ˢ Z ≃ X ×ˢ (Y ×ˢ Z) where
@@ -203,41 +248,107 @@ noncomputable abbrev SetTheory.Set.prod_associator (X Y Z:Set) : (X ×ˢ Y) ×ˢ
 -/
 noncomputable abbrev SetTheory.Set.singleton_iProd_equiv (i:Object) (X:Set) :
     iProd (fun _:({i}:Set) ↦ X) ≃ X where
-  toFun := sorry
-  invFun := sorry
-  left_inv := sorry
-  right_inv := sorry
+  toFun z := mem_iProd z.val |>.mp z.prop |>.choose ⟨i, mem_singleton _ _ |>.mpr rfl⟩ 
+  invFun z := by
+    refine ⟨tuple (fun _:({i}:Set) => z), ?_⟩ 
+    rw [mem_iProd]
+    use fun _ => z
+  left_inv z := by
+    let h := (mem_iProd _).mp z.property
+    obtain ht := h.choose_spec
+    ext
+    rw [ht, tuple_inj]
+    funext i'
+    have : i' = ⟨i, mem_singleton _ _ |>.mpr rfl⟩ := by
+      have : i = ↑i' := mem_singleton _ _ |>.mp i'.prop |>.symm
+      simp [this]
+    simp [this]
+  right_inv  := fun ⟨x, hx⟩ => by
+    dsimp only
+    generalize_proofs h
+    rw [← tuple_inj _ _ |>.mp h.choose_spec]
 
 /-- Example 3.5.10 -/
 abbrev SetTheory.Set.empty_iProd_equiv (X: (∅:Set) → Set) : iProd X ≃ Unit where
-  toFun := sorry
-  invFun := sorry
-  left_inv := sorry
-  right_inv := sorry
+  toFun _ := ()
+  invFun _ := ⟨tuple (absurd ·.prop (not_mem_empty _)), tuple_mem_iProd _⟩ 
+  left_inv x := by
+    dsimp only
+    ext
+    obtain ⟨t, ht⟩ := mem_iProd _ |>.mp x.prop
+    rw [ht, tuple_inj]
+    funext x
+    apply absurd x.prop (not_mem_empty _)
+  right_inv x := rfl
 
-/-- Example 3.5.10 -/
-noncomputable abbrev SetTheory.Set.iProd_of_const_equiv (I:Set) (X: Set) :
-    iProd (fun _:I ↦ X) ≃ (I → X) where
-  toFun := sorry
-  invFun := sorry
-  left_inv := sorry
-  right_inv := sorry
 
+/- open Classical in -/
 /-- Example 3.5.10 -/
 noncomputable abbrev SetTheory.Set.iProd_equiv_prod (X: ({0,1}:Set) → Set) :
     iProd X ≃ (X ⟨ 0, by simp ⟩) ×ˢ (X ⟨ 1, by simp ⟩) where
-  toFun := sorry
-  invFun := sorry
-  left_inv := sorry
-  right_inv := sorry
+  toFun t :=
+    let x := ((mem_iProd _).mp t.property).choose
+    mk_cartesian (x ⟨0, by simp⟩) (x ⟨1, by simp⟩)
+  invFun := fun z ↦ ⟨tuple (X:=X) (fun i ↦ by
+    if h0 : i = ⟨0, by simp⟩ then rw [h0]; exact (fst z)
+    else if h1 : i = ⟨1, by simp⟩ then rw [h1]; exact (snd z)
+    else exact absurd (subtype_pair i |>.resolve_left h0) h1
+  ), by apply tuple_mem_iProd⟩
+  left_inv t := by
+    have h := (mem_iProd _).mp t.property
+    have ht := h.choose_spec
+    ext
+    rw [ht, tuple_inj]
+    ext i
+    if h0 : i = ⟨0, by simp⟩ then
+      rw [dif_pos h0, fst_of_mk_cartesian]
+      subst h0
+      rw [eq_mpr_eq_cast, cast_eq]
+    else if h1 : i = ⟨1, by simp⟩ then
+      rw [dif_neg h0, dif_pos h1, snd_of_mk_cartesian]
+      subst h1
+      rw [eq_mpr_eq_cast, cast_eq]
+    else exact absurd (subtype_pair i |>.resolve_left h0) h1
+  right_inv x := by
+    dsimp only []
+    generalize_proofs _ _ _ _ _ h
+    simp [← tuple_inj _ _ |>.mp h.choose_spec]
 
 /-- Example 3.5.10 -/
 noncomputable abbrev SetTheory.Set.iProd_equiv_prod_triple (X: ({0,1,2}:Set) → Set) :
     iProd X ≃ (X ⟨ 0, by simp ⟩) ×ˢ (X ⟨ 1, by simp ⟩) ×ˢ (X ⟨ 2, by simp ⟩) where
-  toFun := sorry
-  invFun := sorry
-  left_inv := sorry
-  right_inv := sorry
+  toFun t :=
+    let x := ((mem_iProd _).mp t.property).choose
+    mk_cartesian (x ⟨0, by simp⟩) <| mk_cartesian (x ⟨1, by simp⟩) (x ⟨2, by simp⟩)
+  invFun := fun z ↦ ⟨tuple (X:=X) (fun i ↦ by
+    if h0 : i = ⟨0, by simp⟩ then rw [h0]; exact (fst z)
+    else if h1 : i = ⟨1, by simp⟩ then rw [h1]; exact fst (snd z)
+    else if h2 : i = ⟨2, by simp⟩ then rw [h2]; exact snd (snd z)
+    else exact absurd (subtype_triple i |>.resolve_left h0 |>.resolve_left h1) h2
+  ), by apply tuple_mem_iProd⟩
+  left_inv t := by
+    have h := (mem_iProd _).mp t.property
+    have ht := h.choose_spec
+    ext
+    rw [ht, tuple_inj]
+    ext i
+    if h0 : i = ⟨0, by simp⟩ then
+      rw [dif_pos h0, fst_of_mk_cartesian]
+      subst h0
+      rw [eq_mpr_eq_cast, cast_eq]
+    else if h1 : i = ⟨1, by simp⟩ then
+      rw [dif_neg h0, dif_pos h1, snd_of_mk_cartesian, fst_of_mk_cartesian]
+      subst h1
+      rw [eq_mpr_eq_cast, cast_eq]
+    else if h2 : i = ⟨2, by simp⟩ then
+      rw [dif_neg h0, dif_neg h1, dif_pos h2, snd_of_mk_cartesian, snd_of_mk_cartesian]
+      subst h2
+      rw [eq_mpr_eq_cast, cast_eq]
+    else exact absurd (subtype_triple i |>.resolve_left h0 |>.resolve_left h1) h2
+  right_inv x := by
+    dsimp only []
+    generalize_proofs _ _ _ _ _ _ _ h
+    simp [← tuple_inj _ _ |>.mp h.choose_spec]
 
 /-- Connections with Mathlib's `Set.pi` -/
 noncomputable abbrev SetTheory.Set.iProd_equiv_pi (I:Set) (X: I → Set) :
@@ -269,6 +380,17 @@ theorem SetTheory.Set.mem_Fin (n:ℕ) (x:Object) : x ∈ Fin n ↔ ∃ m, m < n 
   intro ⟨ m, hm, h ⟩
   use (by rw [h, ←Object.ofnat_eq]; exact (m:nat).property)
   grind [Object.ofnat_eq''']
+
+theorem SetTheory.Set.Fin_mem_exists (h: n ≠ 0) : ∃m, m ∈ Fin n := by
+  use n.pred
+  rw [mem_Fin]
+  use n.pred
+  simp [Nat.zero_lt_of_ne_zero h]
+
+lemma SetTheory.Set.not_mem_Fin_0 {x : Object} : x ∉ Fin 0 := by
+  intro h
+  have ⟨m, hm, _⟩ := mem_Fin _ _ |>.mp h
+  exact Nat.not_succ_le_zero m hm
 
 abbrev SetTheory.Set.Fin_mk (n m:ℕ) (h: m < n): Fin n := ⟨ m, by rw [mem_Fin]; use m ⟩
 
@@ -365,7 +487,23 @@ theorem SetTheory.Set.finite_choice {n:ℕ} {X: Fin n → Set} (h: ∀ i, X i �
 /-- Exercise 3.5.1, second part (requires axiom of regularity) -/
 abbrev OrderedPair.toObject' : OrderedPair ↪ Object where
   toFun p := ({ p.fst, (({p.fst, p.snd}:Set):Object) }:Set)
-  inj' := by sorry
+  inj' := by 
+    rintro ⟨a1, a2⟩ ⟨b1, b2⟩ h
+    replace h := Function.Embedding.injective _ h
+    simp [pair_eq_iff] at h
+    rw [OrderedPair.eq]
+    rcases h with (⟨rfl, h|h⟩|⟨ha, hb⟩)
+    · exact h
+    · exact ⟨rfl, h.right.trans h.left⟩ 
+    obtain ⟨a1, rfl⟩ : ∃(a: Set), a1 = ↑a := Exists.intro _ ha
+    obtain ⟨b1, rfl⟩ : ∃(a: Set), b1 = ↑a := Exists.intro _ hb.symm
+    replace ha := Function.Embedding.injective _ ha
+    replace hb := Function.Embedding.injective _ hb
+    simp at ha hb
+    exact not_mem_mem a1 b1 |>.elim
+      (fun h => h (hb ▸ mem_pair _ _ _ |>.mpr (Or.inl rfl)))
+      (fun h => h (ha ▸ mem_pair _ _ _ |>.mpr (Or.inl rfl)))
+      |>.elim
 
 /-- An alternate definition of a tuple, used in Exercise 3.5.2 -/
 structure SetTheory.Set.Tuple (n:ℕ) where
@@ -387,115 +525,394 @@ lemma SetTheory.Set.Tuple.ext {n:ℕ} {t t':Tuple n}
 
 /-- Exercise 3.5.2 -/
 theorem SetTheory.Set.Tuple.eq {n:ℕ} (t t':Tuple n) :
-    t = t' ↔ ∀ n : Fin n, ((t.x n):Object) = ((t'.x n):Object) := by sorry
+  t = t' ↔ ∀ n : Fin n, ((t.x n):Object) = ((t'.x n):Object) := by
+    constructor
+    · rintro rfl n
+      rfl
+    rintro h
+    ext i
+    constructor
+    · intro hi
+      have ⟨m, hm⟩ := t.surj ⟨i, hi⟩ 
+      replace h := hm ▸ h m
+      rw [show i = t'.x m from h]
+      exact (t'.x m).prop
+    · intro hi
+      have ⟨m, hm⟩ := t'.surj ⟨i, hi⟩ 
+      replace h := hm ▸ h m |>.symm
+      rw [show i = t.x m from h]
+      exact (t.x m).prop
+    exact h i
 
 noncomputable abbrev SetTheory.Set.iProd_equiv_tuples (n:ℕ) (X: Fin n → Set) :
     iProd X ≃ { t:Tuple n // ∀ i, (t.x i:Object) ∈ X i } where
-  toFun := sorry
-  invFun := sorry
-  left_inv := sorry
-  right_inv := sorry
+  toFun := fun ⟨x, hx⟩ => by
+    have x := mem_iProd _ |>.mp hx |>.choose
+    let X' := iUnion (Fin n) fun i => {(x i: Object)}
+    refine ⟨Tuple.mk X' (fun i => ⟨x i, ?_⟩) ?_, ?_⟩ 
+    · rw [mem_iUnion]
+      use i
+      simp
+    · intro ⟨y, hy⟩ 
+      obtain ⟨z, hz⟩ := mem_iUnion _ _ |>.mp hy
+      use z
+      rw [Subtype.mk.injEq]
+      exact mem_singleton _ _ |>.mp hz |>.symm
+    · intro i
+      simp [x i |>.prop]
+  invFun := fun ⟨t, ht⟩ => by
+    let x (i: Fin n): X i := ⟨t.x i |>.val, ht i⟩ 
+    refine ⟨tuple x, ?_⟩ 
+    rw [mem_iProd]
+    use x
+  left_inv := by
+    intro ⟨t, ht⟩  
+    obtain ht := mem_iProd _ |>.mp ht
+    simp only [Subtype.coe_eta, ← ht.choose_spec]
+  right_inv := by
+    intro ⟨t, ht⟩ 
+    ext i
+    dsimp only
+    generalize_proofs h'
+    have := tuple_inj _ _ |>.mp h'.choose_spec
+    simp only [← this, mem_iUnion, mem_singleton]
+    constructor
+    · intro ⟨a,ha⟩ 
+      exact ha ▸ (t.x a).prop
+    · intro hi
+      obtain ⟨a, ha⟩ := t.surj ⟨i, hi⟩ 
+      use a, ha ▸ rfl
+    simp
+    generalize_proofs h'
+    simp [← tuple_inj _ _ |>.mp h'.choose_spec]
 
 /--
   Exercise 3.5.3. The spirit here is to avoid direct rewrites (which make all of these claims
   trivial), and instead use `OrderedPair.eq` or `SetTheory.Set.tuple_inj`
 -/
-theorem OrderedPair.refl (p: OrderedPair) : p = p := by sorry
+theorem OrderedPair.refl (p: OrderedPair) : p = p := by
+  rw [OrderedPair.eq]
+  grind
 
-theorem OrderedPair.symm (p q: OrderedPair) : p = q ↔ q = p := by sorry
+theorem OrderedPair.symm (p q: OrderedPair) : p = q ↔ q = p := by
+  rw [OrderedPair.eq, OrderedPair.eq]
+  constructor; repeat
+    intro ⟨h1, h2⟩ 
+    exact And.intro h1.symm h2.symm
 
-theorem OrderedPair.trans {p q r: OrderedPair} (hpq: p=q) (hqr: q=r) : p=r := by sorry
+theorem OrderedPair.trans {p q r: OrderedPair} (hpq: p = q) (hqr: q = r) : p = r := by
+  rw [OrderedPair.eq] at hpq hqr ⊢
+  exact ⟨hpq.left.trans hqr.left, hpq.right.trans hqr.right⟩ 
 
 theorem SetTheory.Set.tuple_refl {I:Set} {X: I → Set} (a: ∀ i, X i) :
-    tuple a = tuple a := by sorry
+  tuple a = tuple a := tuple_inj _ _ |>.mpr rfl
 
 theorem SetTheory.Set.tuple_symm {I:Set} {X: I → Set} (a b: ∀ i, X i) :
-    tuple a = tuple b ↔ tuple b = tuple a := by sorry
+  tuple a = tuple b ↔ tuple b = tuple a := by
+    rw [tuple_inj, tuple_inj, eq_comm]
+
 
 theorem SetTheory.Set.tuple_trans {I:Set} {X: I → Set} {a b c: ∀ i, X i}
   (hab: tuple a = tuple b) (hbc : tuple b = tuple c) :
-    tuple a = tuple c := by sorry
+    tuple a = tuple c := by
+      rw [tuple_inj] at hab hbc ⊢
+      exact hab.trans hbc
 
 /-- Exercise 3.5.4 -/
-theorem SetTheory.Set.prod_union (A B C:Set) : A ×ˢ (B ∪ C) = (A ×ˢ B) ∪ (A ×ˢ C) := by sorry
+@[simp]
+theorem SetTheory.Set.prod_union (A B C:Set) : A ×ˢ (B ∪ C) = (A ×ˢ B) ∪ (A ×ˢ C) := by
+  ext x
+  simp_rw [mem_union, mem_cartesian]
+  constructor
+  · rintro ⟨x, ⟨y, hy⟩, rfl⟩ 
+    rcases mem_union _ _ _ |>.mp hy with hy|hy
+    exact Or.inl ⟨x, ⟨y, hy⟩, rfl⟩ 
+    exact Or.inr ⟨x, ⟨y, hy⟩, rfl⟩ 
+  · rintro (⟨x, y, rfl⟩|⟨x, y, rfl⟩ )
+    exact ⟨x, ⟨y, (mem_union _ _ _).mpr (Or.inl y.prop)⟩, rfl⟩ 
+    exact ⟨x, ⟨y, (mem_union _ _ _).mpr (Or.inr y.prop)⟩, rfl⟩ 
+
 
 /-- Exercise 3.5.4 -/
-theorem SetTheory.Set.prod_inter (A B C:Set) : A ×ˢ (B ∩ C) = (A ×ˢ B) ∩ (A ×ˢ C) := by sorry
+@[simp]
+theorem SetTheory.Set.prod_inter (A B C:Set) : A ×ˢ (B ∩ C) = (A ×ˢ B) ∩ (A ×ˢ C) := by
+  ext x
+  simp_rw [mem_inter, mem_cartesian]
+  constructor
+  · rintro ⟨x, ⟨y, hy⟩, rfl⟩ 
+    exact ⟨
+      ⟨x, ⟨y, mem_inter _ _ _  |>.mp hy |>.1⟩, rfl⟩,
+      ⟨x, ⟨y, mem_inter _ _ _  |>.mp hy |>.2⟩, rfl⟩,
+     ⟩ 
+  rintro ⟨⟨x, ⟨y, hyB⟩, rfl⟩, ⟨x', ⟨y', hyC⟩, h⟩⟩
+  replace h := OrderedPair.eq _ _ _ _ |>.mp (Function.Embedding.injective _ h)
+  obtain rfl := Subtype.coe_inj.mp h.left
+  obtain rfl: y = y' := h.right
+  use x, ⟨y, mem_inter _ _ _ |>.mpr ⟨hyB, hyC⟩⟩ 
 
 /-- Exercise 3.5.4 -/
-theorem SetTheory.Set.prod_diff (A B C:Set) : A ×ˢ (B \ C) = (A ×ˢ B) \ (A ×ˢ C) := by sorry
+@[simp]
+theorem SetTheory.Set.prod_diff (A B C:Set) : A ×ˢ (B \ C) = (A ×ˢ B) \ (A ×ˢ C) := by
+  ext x
+  simp_rw [mem_sdiff, mem_cartesian, not_exists]
+  constructor
+  · rintro ⟨x, ⟨y, hy⟩, rfl⟩
+    rw [mem_sdiff] at hy
+    refine ⟨⟨x, ⟨y, hy.left⟩, rfl⟩, ?_⟩ 
+    rintro x' y'
+    by_contra h
+    replace h : y = y' := OrderedPair.eq _ _ _ _ |>.mp (Function.Embedding.injective _ h) |>.right
+    replace h := h ▸ y'.prop
+    exact hy.right h
+  rintro ⟨⟨x, ⟨y, hyB⟩, rfl⟩, h⟩ 
+  by_cases hyC : y ∈ C
+  · have := h x ⟨y, hyC⟩ 
+    contradiction
+  use x, ⟨y, mem_sdiff _ _ _ |>.mpr ⟨hyB, hyC⟩⟩ 
 
 /-- Exercise 3.5.4 -/
-theorem SetTheory.Set.union_prod (A B C:Set) : (A ∪ B) ×ˢ C = (A ×ˢ C) ∪ (B ×ˢ C) := by sorry
+@[simp]
+theorem SetTheory.Set.union_prod (A B C:Set) : (A ∪ B) ×ˢ C = (A ×ˢ C) ∪ (B ×ˢ C) := by aesop
 
 /-- Exercise 3.5.4 -/
-theorem SetTheory.Set.inter_prod (A B C:Set) : (A ∩ B) ×ˢ C = (A ×ˢ C) ∩ (B ×ˢ C) := by sorry
+@[simp]
+theorem SetTheory.Set.inter_prod (A B C:Set) : (A ∩ B) ×ˢ C = (A ×ˢ C) ∩ (B ×ˢ C) := by aesop
 
 /-- Exercise 3.5.4 -/
-theorem SetTheory.Set.diff_prod (A B C:Set) : (A \ B) ×ˢ C = (A ×ˢ C) \ (B ×ˢ C) := by sorry
+@[simp]
+theorem SetTheory.Set.diff_prod (A B C:Set) : (A \ B) ×ˢ C = (A ×ˢ C) \ (B ×ˢ C) := by aesop
 
 /-- Exercise 3.5.5 -/
+@[simp]
 theorem SetTheory.Set.inter_of_prod (A B C D:Set) :
-    (A ×ˢ B) ∩ (C ×ˢ D) = (A ∩ C) ×ˢ (B ∩ D) := by sorry
+  (A ×ˢ B) ∩ (C ×ˢ D) = (A ∩ C) ×ˢ (B ∩ D) := by aesop
+    
+
 
 /- Exercise 3.5.5 -/
 def SetTheory.Set.union_of_prod :
   Decidable (∀ (A B C D:Set), (A ×ˢ B) ∪ (C ×ˢ D) = (A ∪ C) ×ˢ (B ∪ D)) := by
   -- the first line of this construction should be `apply isTrue` or `apply isFalse`.
-  sorry
+  apply isFalse
+  push_neg
+  use {0}, {}, {}, {3}
+  apply not_eq_iff.mpr
+  use OrderedPair.mk 0 3
+  simp
 
 /- Exercise 3.5.5 -/
 def SetTheory.Set.diff_of_prod :
   Decidable (∀ (A B C D:Set), (A ×ˢ B) \ (C ×ˢ D) = (A \ C) ×ˢ (B \ D)) := by
   -- the first line of this construction should be `apply isTrue` or `apply isFalse`.
-  sorry
+  apply isFalse
+  push_neg
+  use {0}, {0, 1}, {0}, {}
+  apply not_eq_iff.mpr
+  use OrderedPair.mk 0 1
+  simp
 
 /--
   Exercise 3.5.6.
 -/
 theorem SetTheory.Set.prod_subset_prod {A B C D:Set}
-  (hA: A ≠ ∅) (hB: B ≠ ∅) (hC: C ≠ ∅) (hD: D ≠ ∅) :
-    A ×ˢ B ⊆ C ×ˢ D ↔ A ⊆ C ∧ B ⊆ D := by sorry
+  (hA: A ≠ ∅) (hB: B ≠ ∅) :
+  A ×ˢ B ⊆ C ×ˢ D ↔ A ⊆ C ∧ B ⊆ D := by
+    constructor
+    · intro h 
+      refine ⟨fun x hx => ?_, fun x hx => ?_⟩ 
+      · have ⟨b, hb⟩ := nonempty_def hB
+        replace h := h (OrderedPair.mk x b) (by simp [hx, hb])
+        replace ⟨x', _, h⟩  := mem_cartesian _ _ _ |>.mp h
+        have : x = x'.val := 
+          Function.Embedding.injective OrderedPair.toObject h 
+          |> (OrderedPair.eq _ _ _ _ |>.mp)
+          |>.left
+        exact this ▸ x'.prop
+      · have ⟨a, ha⟩ := nonempty_def hA
+        replace h := h (OrderedPair.mk a x) (by simp [hx, ha])
+        replace ⟨_, x', h⟩  := mem_cartesian _ _ _ |>.mp h
+        have : x = x'.val := 
+          Function.Embedding.injective OrderedPair.toObject h 
+          |> (OrderedPair.eq _ _ _ _ |>.mp)
+          |>.right
+        exact this ▸ x'.prop
+    intro ⟨hAC, hBD⟩ x hx
+    rw [mem_cartesian] at hx ⊢
+    obtain ⟨⟨a, ha⟩, ⟨b, hb⟩, rfl⟩ := hx
+    use ⟨a, hAC _ ha⟩, ⟨b, hBD _ hb⟩ 
 
 def SetTheory.Set.prod_subset_prod' :
   Decidable (∀ (A B C D:Set), A ×ˢ B ⊆ C ×ˢ D ↔ A ⊆ C ∧ B ⊆ D) := by
   -- the first line of this construction should be `apply isTrue` or `apply isFalse`.
-  sorry
+  apply isFalse
+  push_neg
+  use {0}, {}, {}, {}
+  simp [subset_def]
+
 
 /-- Exercise 3.5.7 -/
 theorem SetTheory.Set.direct_sum {X Y Z:Set} (f: Z → X) (g: Z → Y) :
-    ∃! h: Z → X ×ˢ Y, fst ∘ h = f ∧ snd ∘ h = g := by sorry
+  ∃! h: Z → X ×ˢ Y, fst ∘ h = f ∧ snd ∘ h = g := by
+    apply existsUnique_of_exists_of_unique
+    · refine ⟨fun z => mk_cartesian (f z) (g z), ?_, ?_⟩ <;> funext z <;> simp
+    rintro x1 x2 hx1 hx2 
+    have {x: Z.toSubtype → (X ×ˢ Y).toSubtype} {z} (hx: fst ∘ x = f ∧ snd ∘ x = g) : 
+      x z = mk_cartesian (f z) (g z) := by
+        rw [← mk_cartesian_fst_snd_eq (x z)]
+        simp only [mk_cartesian, Subtype.mk.injEq, EmbeddingLike.apply_eq_iff_eq, OrderedPair.mk.injEq]
+        rw [← Function.comp_apply (f := fst), hx.left, ← Function.comp_apply (f := snd), hx.right]
+        exact And.intro rfl rfl
+    funext z
+    rw [this hx1, this hx2]
 
 /-- Exercise 3.5.8 -/
 @[simp]
 theorem SetTheory.Set.iProd_empty_iff {n:ℕ} {X: Fin n → Set} :
-    iProd X = ∅ ↔ ∃ i, X i = ∅ := by sorry
+  iProd X = ∅ ↔ ∃ i, X i = ∅ := by
+    constructor
+    · intro h
+      simp [eq_empty_iff_forall_notMem] at h
+      by_contra! h'
+      exact h (nonempty_choose <| h' ·)
+    rintro ⟨i, hi⟩ 
+    refine eq_empty_iff_forall_notMem.mpr fun x => ?_
+    rw [mem_iProd]
+    push_neg
+    intro xi
+    exact absurd (hi ▸ xi i |>.prop) (not_mem_empty _)
 
 /-- Exercise 3.5.9-/
 theorem SetTheory.Set.iUnion_inter_iUnion {I J: Set} (A: I → Set) (B: J → Set) :
-    (iUnion I A) ∩ (iUnion J B) = iUnion (I ×ˢ J) (fun p ↦ (A (fst p)) ∩ (B (snd p))) := by sorry
+  (iUnion I A) ∩ (iUnion J B) = iUnion (I ×ˢ J) (fun p ↦ (A (fst p)) ∩ (B (snd p))) := by
+    ext x
+    simp only [mem_inter, mem_iUnion]
+    constructor
+    · rintro ⟨⟨i, ha⟩, ⟨j, hb⟩⟩ 
+      use mk_cartesian i j
+      simp [ha, hb]
+    · rintro ⟨i, ⟨ha, hb⟩⟩ 
+      exact And.intro ⟨fst i, ha⟩ ⟨snd i, hb⟩
+
+theorem SetTheory.Set.iInter_union_iInter {I J: Set} (hI: I ≠ ∅) (hJ: J ≠ ∅) (A: I → Set) (B: J → Set) :
+  (I.iInter hI A) ∪ (J.iInter hJ B) = 
+  iInter (I ×ˢ J) (cartesian_nonempty_iff.mpr ⟨hI, hJ⟩) (fun p ↦ (A (fst p)) ∪ (B (snd p))) := by
+    ext x
+    simp only [mem_union, mem_iInter]
+    constructor
+    · rintro (ha|hb) ⟨i, hi⟩
+      <;> obtain ⟨i, j, rfl⟩ := mem_cartesian _ _ _ |>.mp hi
+      exact Or.inl (fst_of_mk_cartesian _ _ ▸ ha i)
+      exact Or.inr (snd_of_mk_cartesian _ _ ▸ hb j)
+    intro h
+    contrapose! h
+    obtain ⟨⟨i, hi⟩, ⟨j, hj⟩⟩ := h
+    use mk_cartesian i j
+    refine And.intro (fst_of_mk_cartesian _ _ ▸ hi) (snd_of_mk_cartesian _ _ ▸ hj)
 
 abbrev SetTheory.Set.graph {X Y:Set} (f: X → Y) : Set :=
   (X ×ˢ Y).specify (fun p ↦ (f (fst p) = snd p))
 
 /-- Exercise 3.5.10 -/
 theorem SetTheory.Set.graph_inj {X Y:Set} (f f': X → Y) :
-    graph f = graph f' ↔ f = f' := by sorry
+  graph f = graph f' ↔ f = f' := by
+    refine ⟨?_, fun h => h ▸ rfl⟩ 
+    intro h
+    ext x
+    let p := (mk_cartesian x (f x))
+    replace h := Set.ext_iff.mp h p
+    simp_rw [specification_axiom''] at h
+    replace ⟨_, h⟩  := h.mp ⟨p.prop, by simp⟩ 
+    simp at h
+    rw [h]
 
 theorem SetTheory.Set.is_graph {X Y G:Set} (hG: G ⊆ X ×ˢ Y)
   (hvert: ∀ x:X, ∃! y:Y, ((⟨x,y⟩:OrderedPair):Object) ∈ G) :
-    ∃! f: X → Y, G = graph f := by sorry
+  ∃! f: X → Y, G = graph f := by 
+    apply existsUnique_of_exists_of_unique
+    · let g (x: X): Y := hvert x |>.choose
+      use g
+      ext xy
+      rw [specification_axiom'']
+      constructor
+      · intro hxy
+        use hG _ hxy
+        simp [g]
+        generalize_proofs hXY h
+        obtain ⟨x, y, rfl⟩  : ∃x y, xy = mk_cartesian (X := X) (Y := Y) x y := by
+          use fst ⟨_, hXY⟩, snd ⟨_, hXY⟩ 
+          simp
+        replace h := h.choose_spec.right y y.prop (fst_of_mk_cartesian _ _ ▸ hxy)
+        rw [← h, snd_of_mk_cartesian]
+      rintro ⟨hXY, h⟩ 
+      obtain ⟨x, y, rfl⟩  : ∃x y, xy = ↑(mk_cartesian x y) := by
+        use fst ⟨xy, hXY⟩, snd ⟨xy, hXY⟩ 
+        simp
+      simp [g] at h
+      generalize_proofs h' at h
+      exact h ▸ h'.choose_spec.left
+    rintro f1 f2 h rfl
+    exact graph_inj _ _ |>.mp h.symm
 
 /--
   Exercise 3.5.11. This trivially follows from `SetTheory.Set.powerset_axiom`, but the
   exercise is to derive it from `SetTheory.Set.exists_powerset` instead.
 -/
 theorem SetTheory.Set.powerset_axiom' (X Y:Set) :
-    ∃! S:Set, ∀(F:Object), F ∈ S ↔ ∃ f: Y → X, f = F := sorry
+  ∃! S:Set, ∀(F:Object), F ∈ S ↔ ∃ f: Y → X, f = F := by
+    apply existsUnique_of_exists_of_unique
+    · let ⟨Z, hZ⟩ := exists_powerset (Y ×ˢ X)
+      let Z' := Z.specify (fun z =>
+        have := hZ z |>.mp z.prop
+        have G := this.choose
+        ∀ y:Y, ∃! x:X, ((⟨y,x⟩:OrderedPair):Object) ∈ G
+      )
+      let Z'' := Z'.replace (P := fun G' f' => 
+        ∃! f: Y → X, f = f' ∧ (G': Object) = (graph f)
+      ) (by rintro G _ _ ⟨⟨f1, ⟨_, h1⟩⟩, ⟨f2, ⟨_, h2⟩⟩⟩; simp_all [graph_inj])
+      use Z''
+      intro F
+      simp [Z'']
+      constructor
+      · rintro ⟨w, _, ⟨f, ⟨hf, _⟩, _⟩⟩ 
+        use f
+      rintro ⟨f, rfl⟩ 
+      use graph f
+      constructor
+      · simp only [Z', specification_axiom'']
+        constructor
+        · rintro y
+          generalize_proofs h
+          obtain hG := Function.Embedding.injective _ h.choose_spec.left |>.symm
+          rw [hG] at *
+          apply existsUnique_of_exists_of_unique
+          · use f y
+            simp
+          intro x1 x2 hx1 hx2
+          simp_all
+        apply hZ _ |>.mpr
+        refine ⟨graph f, rfl, ?_⟩
+        intro xy hxy
+        obtain ⟨h, _⟩ := specification_axiom'' _ _ |>.mp hxy
+        exact h
+      refine existsUnique_of_exists_of_unique ⟨f, rfl, rfl⟩  ?_
+      intro f1 f2 ⟨hf1, _⟩ ⟨hf2, _⟩
+      exact coe_of_fun_inj _ _ |>.mp <| hf1.trans hf2.symm
+    intro Z1 Z2 h1 h2
+    ext F
+    rw [h1 F, h2 F]
 
 /-- Exercise 3.5.12, with errata from web site incorporated -/
 theorem SetTheory.Set.recursion (X: Set) (f: nat → X → X) (c:X) :
-    ∃! a: nat → X, a 0 = c ∧ ∀ n, a (n + 1:ℕ) = f n (a n) := by sorry
+  ∃! a: nat → X, a 0 = c ∧ ∀ n, a (n + 1:ℕ) = f n (a n) := by
+    apply existsUnique_of_exists_of_unique
+    · let a: ℕ → X := _root_.Nat.rec c (fun n a_n => f n a_n)
+      refine ⟨fun n => a n, ?_, ?_⟩ <;> simp [a]
+    intro a1 a2 ha1 ha2
+    ext n
+    obtain ⟨n, rfl⟩: ∃n': ℕ, n = n' := by use (n: ℕ); rw [nat_equiv_coe_of_coe']
+    induction' n with n ih
+    · rw [show ↑(0: ℕ) = (0: nat) by rfl, ha1.left, ha2.left]
+    rw [ha1.right, ha2.right, Subtype.coe_inj.mp ih]
 
 /-- Exercise 3.5.13 -/
 theorem SetTheory.Set.nat_unique (nat':Set) (zero:nat') (succ:nat' → nat')
@@ -505,18 +922,68 @@ theorem SetTheory.Set.nat_unique (nat':Set) (zero:nat') (succ:nat' → nat')
     ∧ ∀ (n:nat) (n':nat'), f n = n' ↔ f (n+1:ℕ) = succ n' := by
   have nat_coe_eq {m:nat} {n} : (m:ℕ) = n → m = n := by aesop
   have nat_coe_eq_zero {m:nat} : (m:ℕ) = 0 → m = 0 := nat_coe_eq
-  obtain ⟨f, hf⟩ := recursion nat' sorry sorry
+  obtain ⟨f, hf⟩ := recursion nat' (fun n n' => succ n') zero
+  have succ_inj {x y} : succ x = succ y ↔ x = y := by
+    refine ⟨fun h => ?_, fun h => h ▸ rfl⟩ 
+    contrapose! h
+    exact succ_of_ne x y h
+  /- have nonzero_iff {x} : x ≠ zero ↔ ∃y, x = succ y := by -/
+  /-   refine ⟨fun h => ?_, fun h => ?_⟩  -/
+  /-   · revert x -/
+  /-     apply ind -/
+  /-     · exact fun h => absurd rfl h -/
+  /-     intro n _ _ -/
+  /-     use n -/
+  /-   by_contra! h' -/
+  /-   obtain ⟨y, hy⟩ := h' ▸ h -/
+  /-   exact succ_ne y hy.symm -/
   apply existsUnique_of_exists_of_unique
   · use f
-    constructor
-    · constructor
-      · intro x1 x2 heq
-        induction' hx1: (x1:ℕ) with i ih generalizing x1 x2
-        · sorry
-        sorry
-      sorry
-    sorry
-  sorry
-
+    refine ⟨⟨?_, ?_⟩, hf.left.left, ?_⟩ 
+    · intro x1 x2 heq
+      induction' hx1: (x1:ℕ) with i ih generalizing x1 x2
+      · have : x1 = 0 :=  nat_coe_eq hx1
+        subst x1
+        simp [hf.left.left] at heq
+        by_cases h: x2 = 0
+        · exact h.symm
+        obtain ⟨x2', hx2'⟩ := _root_.Nat.exists_eq_succ_of_ne_zero fun a ↦ h (nat_coe_eq a)
+        obtain rfl : x2 = ↑x2'.succ := nat_coe_eq hx2'
+        rw [hf.left.right x2'] at heq
+        exact (succ_ne _ heq.symm).elim
+      obtain rfl := nat_coe_eq hx1; clear hx1
+      rw [hf.left.right i] at heq
+      have : x2 ≠ 0 := by
+        by_contra! h
+        simp [h, hf.left.left] at heq
+        exact succ_ne _ heq
+      have : (x2 : ℕ) ≠ 0 := fun a ↦ this (nat_coe_eq a)
+      obtain ⟨x2, hx2'⟩ := _root_.Nat.exists_eq_succ_of_ne_zero this; clear this
+      obtain rfl := nat_coe_eq hx2'; clear hx2'
+      refine (nat_equiv_inj (i + 1) x2.succ).mpr ?_
+      replace heq: f ↑i = f ↑x2 := by
+        simp [hf.left.right x2, succ_inj] at heq
+        exact heq
+      exact (ih heq (nat_equiv_coe_of_coe _) |> (nat_equiv_inj _ _ |>.mp)) ▸ rfl
+    · apply ind
+      · exact ⟨0, hf.left.left⟩
+      intro y ⟨x, hx⟩ 
+      use (x: ℕ).succ
+      rw [← hx, hf.left.right, nat_equiv_coe_of_coe']
+    · intro x y
+      constructor
+      · rintro rfl
+        rw [hf.left.right, nat_equiv_coe_of_coe']
+      · rintro h
+        rwa [hf.left.right, succ_inj, nat_equiv_coe_of_coe'] at h
+  intro f1 f2 hf1 hf2
+  ext x
+  induction' hx: (x:ℕ) with i ih generalizing x
+  · simp_rw [show x = 0 from nat_coe_eq hx, hf1.right.left, hf2.right.left]
+  simp_rw [show x = ↑(i + 1) from nat_coe_eq hx,
+    nat_equiv_coe_of_coe i ▸ hf1.right.right i (f1 i) |>.mp rfl,
+    nat_equiv_coe_of_coe i ▸ hf2.right.right i (f2 i) |>.mp rfl,
+    ih i (nat_equiv_coe_of_coe i) |> (coe_inj _ _ _ |>.mp)
+  ]
 
 end Chapter3
